reorganize files

Iterator/Pure/Combinators/Take.lean
@@ -1,8 +1,0 @@
-prelude
-import Iterator.Combinators.Take
-import Iterator.Pure.Basic
-
-@[always_inline, inline]
-def Iter.take {α : Type w} {β : Type v} (n : Nat) (it : Iter (α := α) β) :
-    Iter (α := Take α Id β) β :=
-  it.toIterM.take n |>.toPureIter
