Iterator/Combinators.lean
@@ -4,9 +4,9 @@ Released under Apache 2.0 license as described in the file LICENSE.
 Authors: Paul Reichert
 -/
 prelude
+import Iterator.Combinators.Monadic
 import Iterator.Combinators.Drop
 import Iterator.Combinators.FilterMap
 import Iterator.Combinators.FlatMap
-import Iterator.Combinators.MonadLift
 import Iterator.Combinators.Take
 import Iterator.Combinators.Zip
