Iterator/Combinators/Monadic.lean
@@ -1,0 +1,7 @@
+prelude
+import Iterator.Combinators.Monadic.Drop
+import Iterator.Combinators.Monadic.FilterMap
+import Iterator.Combinators.Monadic.FlatMap
+import Iterator.Combinators.Monadic.MonadLift
+import Iterator.Combinators.Monadic.Take
+import Iterator.Combinators.Monadic.Zip
