Iterator/Combinators/Monadic/Drop.lean
@@ -1,0 +1,148 @@
+/-
+Copyright (c) 2025 Lean FRO, LLC. All rights reserved.
+Released under Apache 2.0 license as described in the file LICENSE.
+Authors: Paul Reichert
+-/
+prelude
+import Iterator.Basic
+import Iterator.Consumers.Collect
+import Iterator.Consumers.Loop
+
+/-!
+This file provides the iterator combinator `IterM.drop`.
+-/
+
+variable {α : Type w} {m : Type w → Type w'} {β : Type v}
+
+structure Drop (α : Type w) (m : Type w → Type w') (β : Type v) where
+  remaining : Nat
+  inner : IterM (α := α) m β
+
+/--
+Given an iterator `it` and a natural number `n`, `it.drop n` is an iterator that forwards all of
+`it`'s output values except for the first `n`.
+
+**Marble diagram:**
+
+```text
+it          ---a----b---c--d-e--⊥
+it.drop 3   ---------------d-e--⊥
+
+it          ---a--⊥
+it.drop 3   ------⊥
+```
+
+**Termination properties:**
+
+* `Finite` instance: only if `it` is finite
+* `Productive` instance: only if `it` is productive
+
+_TODO_: prove `Productive`
+
+**Performance:**
+
+Currently, this combinator incurs an additional O(1) cost with each output of `it`, even when the iterator
+does not drop any elements anymore.
+-/
+def IterM.drop (n : Nat) (it : IterM (α := α) m β) :=
+  toIter (Drop.mk n it) m β
+
+inductive Drop.PlausibleStep [Iterator α m β] (it : IterM (α := Drop α m β) m β) :
+    (step : IterStep (IterM (α := Drop α m β) m β) β) → Prop where
+  | drop : ∀ {it' out k}, it.inner.inner.plausible_step (.yield it' out) →
+      it.inner.remaining = k + 1 → PlausibleStep it (.skip (it'.drop k))
+  | skip : ∀ {it'}, it.inner.inner.plausible_step (.skip it') →
+      PlausibleStep it (.skip (it'.drop it.inner.remaining))
+  | done : it.inner.inner.plausible_step .done → PlausibleStep it .done
+  | yield : ∀ {it' out}, it.inner.inner.plausible_step (.yield it' out) →
+      it.inner.remaining = 0 → PlausibleStep it (.yield (it'.drop 0) out)
+
+def Drop.step [Monad m] [Iterator α m β] (it : IterM (α := Drop α m β) m β) :
+    HetT m (IterStep (IterM (α := Drop α m β) m β) β) := do
+  match ← it.inner.inner.stepHet with
+  | .yield it' out =>
+    match it.inner.remaining with
+    | 0 => return .yield (it'.drop 0) out
+    | k + 1 => return .skip (it'.drop k)
+  | .skip it' => return .skip (it'.drop it.inner.remaining)
+  | .done => return .done
+
+theorem Drop.PlausibleStep.char [Monad m] [Iterator α m β] {it : IterM (α := Drop α m β) m β} :
+    Drop.PlausibleStep it = (Drop.step it).property := by
+  ext step
+  simp only [Drop.step, bind, HetT.bindH]
+  constructor
+  · intro h
+    cases h
+    all_goals
+      refine ⟨_, ‹_›, ?_⟩
+      simp_all [pure]
+  · rintro ⟨step, hp, h⟩
+    cases step
+    case yield =>
+      dsimp only at h
+      split at h
+      · cases h
+        exact .yield hp ‹_›
+      · cases h
+        exact .drop hp ‹_›
+    case skip =>
+      cases h
+      exact .skip hp
+    case done =>
+      cases h
+      exact .done hp
+
+instance [Monad m] [Iterator α m β] {it : IterM (α := Drop α m β) m β} :
+    Small.{w} (Subtype <| Drop.PlausibleStep it) := by
+  rw [Drop.PlausibleStep.char]
+  exact (Drop.step it).small
+
+instance Drop.instIterator [Monad m] [Iterator α m β] : Iterator (Drop α m β) m β where
+  plausible_step := Drop.PlausibleStep
+  step_small := inferInstance
+  step it := do
+    match (← it.inner.inner.stepH).inflate (small := _) with
+    | .yield it' out h =>
+      match h' : it.inner.remaining with
+      | 0 => pure <| .deflate <| .yield (it'.drop 0) out (.yield h h')
+      | k + 1 => pure <| .deflate <| .skip (it'.drop k) (.drop h h')
+    | .skip it' h =>
+      pure <| .deflate <| .skip (it'.drop it.inner.remaining) (.skip h)
+    | .done h =>
+      pure <| .deflate <| .done (.done h)
+
+def Drop.rel (m : Type w → Type w') [Iterator α m β] [Finite α m] :
+    IterM (α := Drop α m β) m β → IterM (α := Drop α m β) m β → Prop :=
+  InvImage IterM.TerminationMeasures.Finite.rel (IterM.finitelyManySteps ∘ Drop.inner ∘ IterM.inner)
+
+instance Drop.instFinitenessRelation [Iterator α m β] [Monad m] [Finite α m] :
+    FinitenessRelation (Drop α m β) m where
+  rel := Drop.rel m
+  wf := by
+    apply InvImage.wf
+    exact WellFoundedRelation.wf
+  subrelation {it it'} h := by
+    obtain ⟨step, h, h'⟩ := h
+    cases h'
+    case drop it' h' _ =>
+      cases h
+      apply IterM.TerminationMeasures.Finite.rel_of_yield
+      exact h'
+    case skip it' h' =>
+      cases h
+      apply IterM.TerminationMeasures.Finite.rel_of_skip
+      exact h'
+    case done h' =>
+      cases h
+    case yield it' out h' h'' =>
+      cases h
+      apply IterM.TerminationMeasures.Finite.rel_of_yield
+      exact h'
+
+instance Drop.instIteratorToArray [Monad m] [Iterator α m β] [Finite α m] : IteratorToArray (Drop α m β) m :=
+  .defaultImplementation
+
+instance Drop.instIteratorFor [Monad m] [Monad n] [Iterator α m β] [Finite α m] :
+    IteratorFor (Drop α m β) m n :=
+  .defaultImplementation
