Iterator/Combinators/Monadic/FilterMap.lean
@@ -1,0 +1,310 @@
+/-
+Copyright (c) 2025 Lean FRO, LLC. All rights reserved.
+Released under Apache 2.0 license as described in the file LICENSE.
+Authors: Paul Reichert
+-/
+prelude
+import Iterator.Basic
+import Iterator.Consumers.Collect
+import Iterator.Consumers.Loop
+import Iterator.HetT
+
+/-!
+This file provides iterator combinators for filtering and mapping.
+
+* `IterM.filterMap` either modifies or drops each value based on an option-valued mapping function.
+* `IterM.filter` drops some elements based on a predicate.
+* `IterM.map` modifies each value based on a mapping function
+
+Several variants of these combinators are provided:
+
+* `M` suffix: monadic mapping function
+* `H` suffix: heterogeneous variant that allows switching the monad and the universes.
+-/
+
+section FilterMapMH
+
+universe u' v' u v
+
+@[ext]
+structure FilterMapMH (α : Type w) {β : Type v} {γ : Type v'}
+    {m : Type w → Type w'} (f : β → HetT m (Option γ)) where
+  inner : IterM (α := α) m β
+
+variable {α : Type w} {m : Type w → Type w'} {β : Type v} {γ : Type v'}
+    [Monad m] [Iterator α m β] {f : β → HetT m (Option γ)}
+
+/--
+Given an iterator `it`, a monadic `Option`-valued mapping function `f` and a monad transformation `mf`,
+`it.filterMapMH f mf` is an iterator that applies `f` to each output of `it`. If `f` returns `none`,
+the output is dropped. If it returns `some x`, then the iterator yields `x`.
+
+**Marble diagram (without monadic effects):**
+
+```text
+it                 ---a --b--c --d-e--⊥
+it.filterMapMH     ---a'-----c'-------⊥
+```
+
+(given that `f a = some a'`, `f c = some c'` and `f b = f d = d e = none`)
+
+**Termination properties:**
+
+* `Finite` instance: only if `it` is finite
+* `Productive` instance: not available
+
+**Performance:**
+
+This combinator incurs an additional O(1) cost with each output of `it` in addition to the cost of the monadic effects.
+-/
+@[inline]
+def IterM.filterMapMH [Monad m] [Iterator α m β] (f : β → HetT m (Option γ))
+    (it : IterM (α := α) m β) : IterM (α := FilterMapMH α f) m γ :=
+  toIter ⟨it⟩ m γ
+
+def MapMH (α : Type w) {β : Type v} {γ : Type v'} {m : Type w → Type w'} [Functor m]
+    (f : β → HetT m γ) :=
+  FilterMapMH α (fun b => HetT.mapH some (f b))
+
+inductive FilterMapMH.PlausibleStep (it : IterM (α := FilterMapMH α f) m γ) : (step : IterStep (IterM (α := FilterMapMH α f) m γ) γ) → Prop where
+  | yieldNone : ∀ {it' out}, it.inner.inner.plausible_step (.yield it' out) →
+      (f out).property none → PlausibleStep it (.skip (it'.filterMapMH f))
+  | yieldSome : ∀ {it' out out'}, it.inner.inner.plausible_step (.yield it' out) →
+      (f out).property (some out') → PlausibleStep it (.yield (it'.filterMapMH f) out')
+  | skip : ∀ {it'}, it.inner.inner.plausible_step (.skip it') → PlausibleStep it (.skip (it'.filterMapMH f))
+  | done : it.inner.inner.plausible_step .done → PlausibleStep it .done
+
+def FilterMapMH.step (it : IterM (α := FilterMapMH α f) m γ) :
+    HetT m (IterStep (IterM (α := FilterMapMH α f) m γ) γ) := do
+  it.inner.inner.stepHet.bindH fun
+  | .yield it' out => (f out).bindH fun
+      | none => pure <| .skip (it'.filterMapMH f)
+      | some out' => pure <| .yield (it'.filterMapMH f) out'
+  | .skip it' => pure <| .skip (it'.filterMapMH f)
+  | .done => pure <| .done
+
+theorem FilterMapMH.PlausibleStep.char {it : IterM (α := FilterMapMH α f) m γ} :
+    FilterMapMH.PlausibleStep it = (FilterMapMH.step it).property := by
+  ext step
+  simp only [FilterMapMH.step, HetT.bindH]
+  constructor
+  · intro h
+    cases h
+    case yieldNone it' out h h' =>
+      exact ⟨_, h, _, h', rfl⟩
+    case yieldSome it' out h h' =>
+      exact ⟨_, h, _, h', rfl⟩
+    case skip it' h =>
+      exact ⟨_, h, rfl⟩
+    case done h =>
+      exact ⟨_, h, rfl⟩
+  · rintro ⟨step, hp, h⟩
+    cases step
+    case yield it' out =>
+      obtain ⟨out', h, h'⟩ := h
+      match out' with
+      | none =>
+        cases h'
+        exact .yieldNone hp h
+      | some _ =>
+        cases h'
+        exact .yieldSome hp h
+    case skip it' =>
+      cases h
+      exact .skip hp
+    case done =>
+      cases h
+      exact .done hp
+
+instance [Monad m] {it : IterM (α := FilterMapMH α f) m γ} :
+    Small.{w} (Subtype <| FilterMapMH.PlausibleStep it) := by
+  rw [FilterMapMH.PlausibleStep.char]
+  exact (FilterMapMH.step it).small
+
+instance FilterMapMH.instIterator : Iterator (FilterMapMH α f) m γ where
+  plausible_step := FilterMapMH.PlausibleStep
+  step_small := inferInstance
+  step it := do
+    let step ← it.inner.inner.stepH
+    letI step' := step.inflate (small := _)
+    match step' with
+    | .yield it' out h => do
+      match (← (f out).computation).inflate (small := _) with
+      | ⟨none, h'⟩ => pure <| .deflate <| .skip (it'.filterMapMH f) (.yieldNone h h')
+      | ⟨some out', h'⟩ => pure <| .deflate <| .yield (it'.filterMapMH f) out' (.yieldSome h h')
+    | .skip it' h => pure <| .deflate <| .skip (it'.filterMapMH f) (.skip h)
+    | .done h => pure <| .deflate <| .done (.done h)
+
+instance {f : β → HetT m γ} :
+    Iterator (MapMH α f) m γ :=
+  inferInstanceAs <| Iterator (FilterMapMH α _) m γ
+
+instance FilterMapMH.instFinitenessRelation [Finite α m] : FinitenessRelation (FilterMapMH α f) m where
+  rel := InvImage IterM.plausible_successor_of (FilterMapMH.inner ∘ IterM.inner)
+  wf := InvImage.wf _ Finite.wf
+  subrelation {it it'} h := by
+    obtain ⟨step, h, h'⟩ := h
+    cases h'
+    case yieldNone it' out h' h'' =>
+      cases h
+      exact IterM.plausible_successor_of_yield h'
+    case yieldSome it' out h' h'' =>
+      cases h
+      exact IterM.plausible_successor_of_yield h'
+    case skip it' h' =>
+      cases h
+      exact IterM.plausible_successor_of_skip h'
+    case done h' =>
+      cases h
+
+instance {f : β → HetT m γ} [Finite α m] :
+    Finite (MapMH α f) m :=
+  inferInstanceAs <| Finite (FilterMapMH α _) m
+
+instance {f : β → HetT m γ} [Productive α m] :
+    ProductivenessRelation (MapMH α f) m where
+  rel := InvImage IterM.plausible_skip_successor_of (FilterMapMH.inner ∘ IterM.inner)
+  wf := InvImage.wf _ Productive.wf
+  subrelation {it it'} h := by
+    cases h
+    case yieldNone it' out h h' =>
+      simp at h'
+    case skip it' h =>
+      exact h
+
+instance {f : β → HetT m (Option γ)} [Finite α m] :
+    IteratorToArray (FilterMapMH α f) m :=
+  .defaultImplementation
+
+instance FilterMapMH.instIteratorFor [Monad m] [Monad n]
+    [Iterator α m β] [Finite α m] :
+    IteratorFor (FilterMapMH α f) m n :=
+  .defaultImplementation
+
+/--
+`map` operations allow for a more efficient implementation of `toArray`. For example,
+`array.iter.map f |>.toArray happens in-place if possible.
+-/
+instance {f : β → HetT m γ} [IteratorToArray α m] :
+    IteratorToArray (MapMH α f) m where
+  toArrayMapped g it :=
+    IteratorToArray.toArrayMapped
+      (fun x => do g ((← (f x).computation).inflate (small := _)))
+      it.inner.inner
+
+instance MapMH.instIteratorFor [Monad m] [Monad n]
+    [Iterator α m β] [Finite α m] :
+    IteratorFor (MapMH α f) m n :=
+  .defaultImplementation
+
+/--
+Given an iterator `it`, a monadic mapping function `f` and a monad transformation `mf`,
+`it.mapMH f mf` is an iterator that applies `f` to each output of `it`. If `f` returns `none`,
+the output is dropped. If it returns `some x`, then the iterator yields `x`.
+
+**Marble diagram (without monadic effects):**
+
+```text
+it                 ---a --b --c --d -e --⊥
+it.mapMH           ---a'--b'--c'--d'-e'--⊥
+```
+
+(given that `f a = a'` and so on)
+
+**Termination properties:**
+
+* `Finite` instance: only if `it` is finite
+* `Productive` instance: only if `it` is productive
+
+_TODO_: prove `Productive`. This requires us to wrap the FilterMapMH into a new type.
+
+**Performance:**
+
+This combinator incurs an additional O(1) cost with each output of `it` in addition to the cost of the monadic effects.
+-/
+@[inline]
+def IterM.mapMH [Monad m] [Iterator α m β] (f : β → HetT m γ) (it : IterM (α := α) m β) :
+    IterM (α := MapMH α f) m γ :=
+  toIter ⟨it⟩ m γ
+
+/--
+Given an iterator `it`, a monadic predicate `p` and a monad transformation `mf`,
+`it.filterMH p mf` is an iterator that applies `p` to each output of `it`. If `p` returns `false`,
+the output is dropped. Otherwise, the iterator forwards the output of `it`.
+
+**Marble diagram (without monadic effects):**
+
+```text
+it                 ---a--b--c--d-e--⊥
+it.filterMH        ---a-----c-------⊥
+```
+
+(given that `f a = f c = true'` and `f b = f d = d e = false`)
+
+**Termination properties:**
+
+* `Finite` instance: only if `it` is finite
+* `Productive` instance: not available
+
+**Performance:**
+
+This combinator incurs an additional O(1) cost with each output of `it` in addition to the cost of the monadic effects.
+-/
+@[inline]
+def IterM.filterMH [Monad m] [Iterator α m β] (f : β → HetT m Bool) (it : IterM (α := α) m β) :=
+  (it.filterMapMH (fun b => (f b).mapH (fun x => if x = true then some b else none)) : IterM m β)
+
+end FilterMapMH
+
+section FilterMapH
+
+universe u' v' u v
+
+variable {α : Type w} {β : Type v} {m : Type w → Type w'} [Monad m] [Iterator α m β]
+    {γ : Type v'} {f : β → Option γ} [Small.{w} γ]
+
+@[inline]
+def IterM.filterMapH (f : β → Option γ) (it : IterM (α := α) m β) :=
+  (it.filterMapMH (fun b => pure (f b)) : IterM m γ)
+
+@[inline]
+def IterM.mapH (f : β → γ) (it : IterM (α := α) m β) :=
+  (it.mapMH (fun b => pure (f b)) : IterM m γ)
+
+end FilterMapH
+
+section FilterMap
+
+variable {m : Type w → Type w'} {α : Type w} {β : Type v} {γ : Type w} {f : β → Option γ}
+
+@[inline]
+def IterM.filterMap [Iterator α m β] [Monad m] (f : β → Option γ) (it : IterM (α := α) m β) :=
+  (it.filterMapH f : IterM m γ)
+
+@[inline]
+def IterM.map [Iterator α m β] [Monad m] (f : β → γ) (it : IterM (α := α) m β) :=
+  (it.mapH f : IterM m γ)
+
+@[inline]
+def IterM.filter [Iterator α m β] [Monad m] (f : β → Bool) (it : IterM (α := α) m β) :=
+  (it.filterMapH (fun b => if f b then some b else none) : IterM m β)
+
+end FilterMap
+
+section FilterMapM
+
+variable {m : Type w → Type w'} {α : Type w} {β : Type v} {γ : Type w} {f : β → Option γ}
+
+@[inline]
+def IterM.filterMapM [Iterator α m β] [Monad m] (f : β → m (Option γ)) (it : IterM (α := α) m β) :=
+  (it.filterMapMH (fun b => monadLift (f b)) : IterM m γ)
+
+@[inline]
+def IterM.mapM [Iterator α m β] [Monad m] (f : β → m γ) (it : IterM (α := α) m β) :=
+  (it.filterMapMH (fun b => some <$> monadLift (f b)) : IterM m γ)
+
+@[inline]
+def IterM.filterM [Iterator α m β] [Monad m] (f : β → m (USquash Bool)) (it : IterM (α := α) m β) :=
+  (it.filterMapMH (fun b => (HetT.liftSquashed (f b)).mapH (if · = true then some b else none)) : IterM m β)
+
+end FilterMapM
