Iterator/Combinators/Monadic/Take.lean
@@ -1,0 +1,192 @@
+/-
+Copyright (c) 2025 Lean FRO, LLC. All rights reserved.
+Released under Apache 2.0 license as described in the file LICENSE.
+Authors: Paul Reichert
+-/
+prelude
+import Iterator.Basic
+import Iterator.Consumers.Collect
+import Iterator.Consumers.Loop
+import Iterator.HetT
+
+/-!
+This file provides the iterator combinator `IterM.take`.
+-/
+
+variable {α : Type w} {m : Type w → Type w'} {β : Type v}
+
+structure Take (α : Type w) (m : Type w → Type w') (β : Type v) where
+  remaining : Nat
+  inner : IterM (α := α) m β
+
+/--
+Given an iterator `it` and a natural number `n`, `it.take n` is an iterator that outputs
+up to the first `n` of `it`'s values in order and then terminates.
+
+**Marble diagram:**
+
+```text
+it          ---a----b---c--d-e--⊥
+it.take 3   ---a----b---c⊥
+
+it          ---a--⊥
+it.take 3   ---a--⊥
+```
+
+**Termination properties:**
+
+* `Finite` instance: always ✓
+* `Productive` instance: only if `it` is productive
+
+_TODO_: prove `Productive`
+
+**Performance:**
+
+This combinator incurs an additional O(1) cost with each output of `it`.
+-/
+@[inline]
+def IterM.take (n : Nat) (it : IterM (α := α) m β) :=
+  toIter (Take.mk n it) m β
+
+theorem IterM.take.surjective {α : Type w} {m : Type w → Type w'} {β : Type v}
+    (it : IterM (α := Take α m β) m β) :
+    ∃ (it₀ : IterM (α := α) m β) (k : Nat), it = it₀.take k := by
+  refine ⟨it.inner.inner, it.inner.remaining, rfl⟩
+
+inductive Take.PlausibleStep [Iterator α m β] (it : IterM (α := Take α m β) m β) :
+    (step : IterStep (IterM (α := Take α m β) m β) β) → Prop where
+  | yield : ∀ {it' out k}, it.inner.inner.plausible_step (.yield it' out) →
+      it.inner.remaining = k + 1 → PlausibleStep it (.yield (it'.take k) out)
+  | skip : ∀ {it' k}, it.inner.inner.plausible_step (.skip it') →
+      it.inner.remaining = k + 1 → PlausibleStep it (.skip (it'.take (k + 1)))
+  | done : it.inner.inner.plausible_step .done → PlausibleStep it .done
+  | depleted : it.inner.remaining = 0 →
+      PlausibleStep it .done
+
+def Take.step [Monad m] [Iterator α m β] (it : IterM (α := Take α m β) m β) :
+    HetT m (IterStep (IterM (α := Take α m β) m β) β) :=
+  match it.inner.remaining with
+  | 0 => pure .done
+  | k + 1 => do
+    match (← it.inner.inner.stepHet) with
+    | .yield it' out => return .yield (it'.take k) out
+    | .skip it' => return .skip (it'.take (k + 1))
+    | .done => return .done
+
+theorem Take.PlausibleStep.char [Monad m] [Iterator α m β] {it : IterM (α := Take α m β) m β} :
+    Take.PlausibleStep it = (Take.step it).property := by
+  ext step
+  simp only [Take.step]
+  split
+  · simp only [pure]
+    constructor
+    · intro h
+      cases h <;> (try omega; done) <;> rfl
+    · rintro rfl
+      exact .depleted ‹_›
+  · simp [bind, HetT.bindH, IterM.stepHet]
+    constructor
+    · intro h
+      cases h
+      case yield =>
+        refine ⟨_, ‹_›, ?_⟩
+        simp_all [pure]
+      case skip =>
+        refine ⟨_, ‹_›, ?_⟩
+        simp_all [pure]
+      case done =>
+        refine ⟨_, ‹_›, ?_⟩
+        simp_all [pure]
+      case depleted =>
+        omega
+    · rintro ⟨step, hp, h⟩
+      cases step
+      · cases h
+        exact .yield hp ‹_›
+      · cases h
+        exact .skip hp ‹_›
+      · cases h
+        exact .done hp
+
+instance [Iterator α m β] [Monad m] {it : IterM (α := Take α m β) m β} :
+    Small.{w} (Subtype <| Take.PlausibleStep it) := by
+  rw [Take.PlausibleStep.char]
+  exact (Take.step it).small
+
+instance Take.instIterator [Monad m] [Iterator α m β] : Iterator (Take α m β) m β where
+  plausible_step := Take.PlausibleStep
+  step_small := inferInstance
+  step it :=
+    match h : it.inner.remaining with
+    | 0 => pure <| .deflate <| .done (.depleted h)
+    | k + 1 => do
+      match (← it.inner.inner.stepH).inflate (small := _) with
+      | .yield it' out h' => pure <| .deflate <| .yield (it'.take k) out (.yield h' h)
+      | .skip it' h' => pure <| .deflate <| .skip (it'.take (k + 1)) (.skip h' h)
+      | .done h' => pure <| .deflate <| .done (.done h')
+
+def Take.rel (m : Type w → Type w') [Monad m] [Iterator α m β] [Productive α m] :
+    IterM (α := Take α m β) m β → IterM (α := Take α m β) m β → Prop :=
+  InvImage (Prod.Lex Nat.lt_wfRel.rel IterM.TerminationMeasures.Productive.rel)
+    (fun it => (it.inner.remaining, it.inner.inner.finitelyManySkips))
+
+theorem Take.rel_of_remaining [Monad m] [Iterator α m β] [Productive α m] {it it' : IterM (α := Take α m β) m β}
+    (h : it'.inner.remaining < it.inner.remaining) : Take.rel m it' it :=
+  Prod.Lex.left _ _ h
+
+theorem Take.rel_of_inner [Monad m] [Iterator α m β] [Productive α m] {remaining : Nat} {it it' : IterM (α := α) m β}
+    (h : it'.finitelyManySkips.rel it.finitelyManySkips) :
+    Take.rel m (it'.take remaining) (it.take remaining) :=
+  Prod.Lex.right _ h
+
+instance Take.instFinitenessRelation [Monad m] [Iterator α m β] [Productive α m] :
+    FinitenessRelation (Take α m β) m where
+  rel := Take.rel m
+  wf := by
+    apply InvImage.wf
+    refine ⟨fun (a, b) => Prod.lexAccessible (WellFounded.apply ?_ a) (WellFounded.apply ?_) b⟩
+    · exact WellFoundedRelation.wf
+    · exact WellFoundedRelation.wf
+  subrelation {it it'} h := by
+    obtain ⟨step, h, h'⟩ := h
+    cases h'
+    case yield it' out k h' h'' =>
+      cases h
+      apply rel_of_remaining
+      simp_all [IterM.take]
+    case skip it' out k h' h'' =>
+      cases h
+      obtain ⟨it, k, rfl⟩ := IterM.take.surjective it
+      cases h''
+      apply Take.rel_of_inner
+      exact IterM.TerminationMeasures.Productive.rel_of_skip h'
+    case done _ =>
+      cases h
+    case depleted _ =>
+      cases h
+
+instance Take.instIteratorToArray [Monad m] [Iterator α m β] [Productive α m] : IteratorToArray (Take α m β) m :=
+  .defaultImplementation
+
+instance Take.instIteratorFor [Monad m] [Monad n] [Iterator α m β] [Finite α m] :
+    IteratorFor (Take α m β) m n :=
+  .defaultImplementation
+  -- TODO: use [IteratorFor α m n]
+    -- forIn {γ} it init successor_of stepper _ := by
+    -- refine Prod.fst <$> (IteratorFor.forIn (α := α) (m := m) (n := n) (innerIter it) (γ := γ × Nat) (init, it.inner.remaining)
+    --   (successor_of := fun b c c' => c.snd = c'.snd + 1) ?_ ?_)
+    -- · exact fun b c => do
+    --     let result ← stepper b c.fst
+    --     return match result.val with
+    --     | .yield x => .yield ⟨
+    --     | .done x => sorry
+    -- refine Subrelation.wf (r := InvImage IterM.TerminationMeasures.Finite.rel (fun p => (p.1).finitelyManySteps)) ?_ ?_
+    -- · intro p' p h
+    --   cases h
+    --   · apply IterM.plausible_successor_of_skip
+    --     rename_i h
+    --     exact h.1
+    --   · rename_i h
+    --     obtain ⟨out, h, _⟩ := h -- Interesting: Moving `obtain` after `apply` leads to failure
+    --     apply IterM.plausible_successor_of_yield
+    --     exact h
