Iterator/Consumers/Collect.lean
@@ -1,64 +1,23 @@
-import Iterator.Basic
-
-section ToArray
-
-@[always_inline, inline]
-def IterM.DefaultConsumers.toArrayMapped {α : Type w} {m : Type w → Type w'} [Monad m] {β : Type v}
-    {instIt : Iterator α m β} [Finite α m] {γ : Type w} (f : β → m γ) (it : IterM (α := α) m β) : m (Array γ) :=
-  go it #[]
-where
-  @[specialize]
-  go [Monad m] [Finite α m] (it : IterM (α := α) m β) a := do
-    match (← it.stepH).inflate with
-    | .yield it' b _ => go it' (a.push (← f b))
-    | .skip it' _ => go it' a
-    | .done _ => return a
-  termination_by it.finitelyManySteps
-
-class IteratorToArray (α : Type w) (m : Type w → Type w') {β : Type v} [Iterator α m β] where
-  toArrayMapped : ∀ {γ : Type w}, (β → m γ) → IterM (α := α) m β → m (Array γ)
-
-class LawfulIteratorToArray (α : Type w) (m : Type w → Type w') [Monad m] [Iterator α m β] [IteratorToArray α m] where
-  finite : Finite α m
-  lawful : ∀ γ, IteratorToArray.toArrayMapped (α := α) (m := m) (β := β) (γ := γ) =
-    IterM.DefaultConsumers.toArrayMapped (α := α) (m := m) (γ := γ)
-
-instance (α : Type w) (m : Type w → Type w') [Monad m] [Iterator α m β] [IteratorToArray α m]
-    [LawfulIteratorToArray α m] : Finite α m :=
-  LawfulIteratorToArray.finite
-
-def IteratorToArray.defaultImplementation {α : Type w} {m : Type w → Type w'}
-    [Monad m] [Iterator α m β] [Finite α m] : IteratorToArray α m where
-  toArrayMapped := IterM.DefaultConsumers.toArrayMapped
-
-instance (α : Type w) (m : Type w → Type w') [Monad m] [Iterator α m β]
-    [Monad m] [Iterator α m β] [Finite α m] :
-    haveI : IteratorToArray α m := .defaultImplementation
-    LawfulIteratorToArray α m :=
-  letI : IteratorToArray α m := .defaultImplementation
-  ⟨inferInstance, fun _ => rfl⟩
+/-
+Copyright (c) 2025 Lean FRO, LLC. All rights reserved.
+Released under Apache 2.0 license as described in the file LICENSE.
+Authors: Paul Reichert
+-/
+prelude
+import Iterator.Pure
+import Iterator.Consumers.Monadic.Collect
 
 @[always_inline, inline]
-def IterM.toArray {α : Type w} {m : Type w → Type w'} {β : Type w} [Monad m]
-    [Iterator α m β] (it : IterM (α := α) m β) [IteratorToArray α m] : m (Array β) :=
-  IteratorToArray.toArrayMapped pure it
+def Iter.toArray {α : Type w} {β : Type w}
+    [Iterator α Id β] [IteratorToArray α Id] (it : Iter (α := α) β) : Array β :=
+  it.toIterM.toArray
 
-end ToArray
+@[always_inline, inline]
+def Iter.reverseToList {α : Type w} {β : Type w}
+    [Iterator α Id β] [Finite α Id] (it : Iter (α := α) β) : List β :=
+  it.toIterM.reverseToList
 
-@[inline]
-def IterM.reverseToList {α : Type w} {m : Type w → Type w'} [Monad m] {β : Type w}
-    [Iterator α m β] [Finite α m] (it : IterM (α := α) m β) : m (List β) :=
-  go it []
-where
-  @[specialize]
-  go [Finite α m] it bs := do
-    match ← it.step with
-    | .yield it' b _ => go it' (b :: bs)
-    | .skip it' _ => go it' bs
-    | .done _ => return bs
-  termination_by it.finitelyManySteps
-
-@[inline]
-def IterM.toList {α : Type w} {m : Type w → Type w'} [Monad m] {β : Type w}
-    [Iterator α m β] (it : IterM (α := α) m β) [IteratorToArray α m] : m (List β) :=
-  Array.toList <$> IterM.toArray it
+@[always_inline, inline]
+def Iter.toList {α : Type w} {β : Type w}
+    [Iterator α Id β] [IteratorToArray α Id] (it : Iter (α := α) β) : List β :=
+  it.toIterM.toList
