Iterator/Consumers/Loop.lean
@@ -1,85 +1,26 @@
-import Iterator.Basic
+/-
+Copyright (c) 2025 Lean FRO, LLC. All rights reserved.
+Released under Apache 2.0 license as described in the file LICENSE.
+Authors: Paul Reichert
+-/
+prelude
+import Iterator.Pure
+import Iterator.Consumers.Monadic.Loop
 
-@[specialize]
-def IterM.DefaultConsumers.forIn {m : Type w → Type w'}
-    {n : Type w → Type w''} [Monad n] (lift : ∀ γ, m γ → n γ)
-    {α : Type w} {β : Type v} {γ : Type w}
-    [Iterator α m β] [Finite α m]
-    (it : IterM (α := α) m β) (init : γ)
-    (f : (b : β) → (c : γ) → n (ForInStep γ)) : n γ :=
-  letI : MonadLift m n := ⟨fun {γ} => lift γ⟩
-  do
-    match (← it.stepH).inflate with
-    | .yield it' out _ =>
-      match ← f out init with
-      | .yield c => IterM.DefaultConsumers.forIn lift it' c f
-      | .done c => return c
-    | .skip it' _ => IterM.DefaultConsumers.forIn lift it' init f
-    | .done _ => return init
-termination_by it.finitelyManySteps
+instance (α : Type w) (β : Type v) (n : Type w → Type w')
+    [Iterator α Id β] :
+    [IteratorFor α Id n] →
+    ForIn n (Iter (α := α) β) β where
+  forIn it := IteratorFor.forIn (_lift := fun _ c => pure c.run) it.toIterM
 
-class IteratorFor (α : Type w) (m : Type w → Type w') {β : Type v} [Iterator α m β]
-    (n : Type w → Type w'') where
-  forIn : ∀ (_lift : (γ : Type w) → m γ → n γ) {γ : Type w},
-      IterM (α := α) m β → γ →
-      ((b : β) → (c : γ) → n (ForInStep γ)) → n γ
-
-class LawfulIteratorFor (α : Type w) (m : Type w → Type w') (n : Type w → Type w'')
-    [Monad n] [Iterator α m β] [Finite α m] [IteratorFor α m n] where
-  lawful : ∀ lift γ, IteratorFor.forIn lift (α := α) (m := m) (γ := γ) =
-    IterM.DefaultConsumers.forIn (α := α) (m := m) (n := n) (lift := lift) (γ := γ)
-
-def IteratorFor.defaultImplementation {α : Type w} {m : Type w → Type w'} {n : Type w → Type w'}
-    [Monad m] [Monad n] [Iterator α m β] [Finite α m] :
-    IteratorFor α m n where
-  forIn lift := IterM.DefaultConsumers.forIn lift
-
-instance (α : Type w) (m : Type w → Type w') (n : Type w → Type w')
-    [Monad m] [Monad n] [Iterator α m β] [Finite α m] :
-    letI : IteratorFor α m n := .defaultImplementation
-    LawfulIteratorFor α m n :=
-  letI : IteratorFor α m n := .defaultImplementation
-  ⟨fun _ _ => rfl⟩
-
-instance {m : Type w → Type w'} {n : Type w → Type w''}
-    {α : Type w} {β : Type v} [Iterator α m β] [IteratorFor α m n]
-    [MonadLiftT m n] :
-    ForIn n (IterM (α := α) m β) β where
-  forIn := IteratorFor.forIn (fun _ => MonadLiftT.monadLift)
-
-@[specialize]
-def IterM.foldM {m : Type w → Type w'} {n : Type w → Type w'} [Monad n]
-    {α : Type w} {β : Type v} {γ : Type w} [Iterator α m β] [IteratorFor α m n]
-    [MonadLiftT m n]
-    (f : γ → β → n γ) (init : γ) (it : IterM (α := α) m β) : n γ :=
+@[always_inline, inline]
+def Iter.foldM {n : Type w → Type w} [Monad n]
+    {α : Type w} {β : Type v} {γ : Type w} [Iterator α Id β]
+    [IteratorFor α Id n] (f : γ → β → n γ)
+    (init : γ) (it : Iter (α := α) β) : n γ :=
   ForIn.forIn it init (fun x acc => ForInStep.yield <$> f acc x)
 
-@[specialize]
-def IterM.count {α : Type u} {β : Type v} [Iterator α Id β] [Finite α Id]
-    (it : IterM (α := α) Id β) : Nat :=
-  go it 0
-where
-  go [Finite α Id] it acc :=
-    match it.stepH.inflate with
-    | .yield it' _ _ => go it' (acc + 1)
-    | .skip it' _ => go it' acc
-    | .done _ => acc
-  termination_by it.finitelyManySteps
-
-@[specialize]
-def IterM.countM {m : Type → Type w'} [Monad m] {α : Type} {β : Type v} [Iterator α m β] [Finite α m]
-    (it : IterM (α := α) m β) : m Nat :=
-  go it 0
-where
-  go [Finite α m] it acc := do
-    match (← it.stepH).inflate with
-      | .yield it' _ _ => go it' (acc + 1)
-      | .skip it' _ => go it' acc
-      | .done _ => return acc
-  termination_by it.finitelyManySteps
-
-@[specialize]
-def IterM.drain {α : Type w} {m : Type w → Type w'} [Monad m] {β : Type v}
-    [Iterator α m β] [Finite α m] (it : IterM (α := α) m β) [IteratorFor α m m] :
-    m PUnit :=
-  it.foldM (γ := PUnit) (fun _ _ => pure .unit) .unit
+@[always_inline, inline]
+def Iter.count {α : Type u} {β : Type v} [Iterator α Id β] [Finite α Id]
+    (it : Iter (α := α) β) : Nat :=
+  it.toIterM.count
