Iterator/Consumers/Monadic.lean
@@ -4,6 +4,6 @@ Released under Apache 2.0 license as described in the file LICENSE.
 Authors: Paul Reichert
 -/
 prelude
-import Iterator.Consumers.Monadic
-import Iterator.Consumers.Collect
-import Iterator.Consumers.Loop
+import Iterator.Consumers.Monadic.Collect
+import Iterator.Consumers.Monadic.Loop
+import Iterator.Consumers.Monadic.Size
