Iterator/Consumers/Monadic/Size.lean
@@ -4,3 +4,7 @@ Released under Apache 2.0 license as described in the file LICENSE.
 Authors: Paul Reichert
 -/
 prelude
+import Iterator.Basic
+
+class IteratorSized (α : Type u) (m : Type w → Type w') where
+  size : α → Option Nat
