Iterator/Consumers/Size.lean
@@ -1,4 +1,0 @@
-import Iterator.Basic
-
-class IteratorSized (α : Type u) (m : Type w → Type w') where
-  size : α → Option Nat
