Iterator/Lemmas/Monadic.lean
@@ -1,0 +1,11 @@
+/-
+Copyright (c) 2025 Lean FRO, LLC. All rights reserved.
+Released under Apache 2.0 license as described in the file LICENSE.
+Authors: Paul Reichert
+-/
+prelude
+import Iterator.Lemmas.Monadic.Consumer
+import Iterator.Lemmas.Monadic.Equivalence
+import Iterator.Lemmas.Monadic.FilterMap
+import Iterator.Lemmas.Monadic.FlatMap
+import Iterator.Lemmas.Monadic.Producer
