Iterator/Lemmas/Monadic/Producer.lean
@@ -1,3 +1,9 @@
+/-
+Copyright (c) 2025 Lean FRO, LLC. All rights reserved.
+Released under Apache 2.0 license as described in the file LICENSE.
+Authors: Paul Reichert
+-/
+prelude
 import Iterator.Producers
 import Iterator.Consumers
 import Iterator.Lemmas.Monadic.Consumer
