Iterator/Pure/Combinators.lean
@@ -1,6 +1,0 @@
-prelude
-import Iterator.Pure.Combinators.Drop
-import Iterator.Pure.Combinators.FilterMap
-import Iterator.Pure.Combinators.FlatMap
-import Iterator.Pure.Combinators.Take
-import Iterator.Pure.Combinators.Zip
