Iterator/Pure/Combinators/Zip.lean
@@ -1,9 +1,0 @@
-prelude
-import Iterator.Combinators.Zip
-import Iterator.Pure.Basic
-
-@[always_inline, inline]
-def Iter.zip {α₁ : Type w} {β₁: Type v₁} {α₂ : Type w} {β₂ : Type v₂}
-    [Iterator α₁ Id β₁] [Iterator α₂ Id β₂]
-    (left : Iter (α := α₁) β₁) (right : Iter (α := α₂) β₂) :=
-  ((left.toIterM.zipH right.toIterM).toPureIter : Iter (β₁ × β₂))
