Iterator/Pure/Consumers.lean
@@ -1,3 +1,0 @@
-prelude
-import Iterator.Pure.Consumers.Collect
-import Iterator.Pure.Consumers.Loop
